\documentclass{article}

\begin{document}

\section*{Bucket problem}

I started with the change in potential energy for a change in height $\Delta h$:
$$ \Delta PE = \rho * g * A * h^2 - \rho * g * A * (h - \Delta h)^2 = \rho * g * A (h^2 - (h^2 - 2 * h * \Delta hÂ + \Delta h^2))$$
We can simplify $\Delta PE$ to
$$ \Delta PE = \rho * g * A (2* h* \Delta h + \Delta h^2) $$
From here, we can note that the change in potential energy is equal to the kinetic energy leaving the bucket:
$$ KE = (1/2) * \rho * A * \Delta h * v^2 $$
Then, setting $\Delta PE = KE$, we get
$$ \rho * g * A (2* h* \Delta h + \Delta h^2) = (1/2) * \rho * A * \Delta h * v^2 $$
$$ 2 * g * h* \Delta h + g * \Delta h^2 = (1/2)*\Delta h * v^2 $$
$$ 4 * g * h + g * \Delta h = v^2 $$
As we let $\Delta h$ approach 0, we just get
$$ v^2 = 4*g*h $$
I can't seem to find where I went wrong, let me know what you see.
Thanks Tomas!

\end{document}
